- finish d_sub_elab_lc_fexp

proof/uni/decl/prop_safety.v
@@ -16,33 +16,33 @@ Notation "Ψ ⊢ e : A" :=
   (f_typing Ψ e A) 
     (at level 65, e at next level, no associativity) : type_scope.
 
-Fixpoint trans_typ (A : typ) : ftyp :=
+Fixpoint trans_ftyp (A : typ) : ftyp :=
   match A with
   | typ_unit => ftyp_unit
   | typ_top => ftyp_unit
   | typ_bot => ftyp_all (ftyp_var_b 0)
   | typ_var_b n => ftyp_var_b n
   | typ_var_f X => ftyp_var_f X
-  | typ_arrow A1 A2 => ftyp_arrow (trans_typ A1) (trans_typ A2)
-  | typ_all A => ftyp_all (trans_typ A)
-  | typ_union A1 A2 => ftyp_sum (trans_typ A1) (trans_typ A2)
-  | typ_intersection A1 A2 => ftyp_prod (trans_typ A1) (trans_typ A2) 
+  | typ_arrow A1 A2 => ftyp_arrow (trans_ftyp A1) (trans_ftyp A2)
+  | typ_all A => ftyp_all (trans_ftyp A)
+  | typ_union A1 A2 => ftyp_sum (trans_ftyp A1) (trans_ftyp A2)
+  | typ_intersection A1 A2 => ftyp_prod (trans_ftyp A1) (trans_ftyp A2) 
   end.
 
-Notation "ᵗ⟦  A  ⟧" := (trans_typ A) (at level 0, no associativity) : type_scope.
+Notation "ᵗ⟦  A  ⟧" := (trans_ftyp A) (at level 0, no associativity) : type_scope.
 
 Fixpoint trans_env (Ψ : denv) : fenv :=
   match Ψ with
   | nil => nil
   | (X, dbind_tvar_empty) :: Ψ' => (X, fbind_tvar_empty) :: trans_env Ψ'
   | (X, dbind_stvar_empty) :: Ψ' => (X, fbind_tvar_empty) :: trans_env Ψ'
-  | (X, (dbind_typ T)) :: Ψ' => (X, (fbind_typ (trans_typ T))) :: trans_env Ψ'
+  | (X, (dbind_typ T)) :: Ψ' => (X, (fbind_typ (trans_ftyp T))) :: trans_env Ψ'
   end.
 
 Notation "⟦ Ψ ⟧" := (trans_env Ψ) (at level 0, no associativity) : type_scope.
 
-Lemma trans_typ_open_typ_wrt_typ_rec : forall A1 A2 n,
-  trans_typ (open_typ_wrt_typ_rec n A2 A1) = open_ftyp_wrt_ftyp_rec n ᵗ⟦ A2 ⟧ ᵗ⟦ A1 ⟧.
+Lemma trans_ftyp_open_typ_wrt_typ_rec : forall A1 A2 n,
+  trans_ftyp (open_typ_wrt_typ_rec n A2 A1) = open_ftyp_wrt_ftyp_rec n ᵗ⟦ A2 ⟧ ᵗ⟦ A1 ⟧.
 Proof.
   intros A1. induction A1; auto; intros; simpl.
   - destruct (lt_eq_lt_dec n n0) as [[? | ?] | ?] eqn:Ψ; auto.
@@ -52,24 +52,24 @@ Proof.
   - rewrite IHA1_1. rewrite IHA1_2. auto.
 Qed.
 
-Theorem trans_typ_open_typ_wrt_typ : forall A1 A2,
-  trans_typ (A1 ᵗ^^ₜ A2) = open_ftyp_wrt_ftyp (trans_typ A1) (trans_typ A2).
+Theorem trans_ftyp_open_typ_wrt_typ : forall A1 A2,
+  trans_ftyp (A1 ᵗ^^ₜ A2) = open_ftyp_wrt_ftyp (trans_ftyp A1) (trans_ftyp A2).
 Proof.
   unfold open_typ_wrt_typ. unfold open_ftyp_wrt_ftyp.
-  intros. apply trans_typ_open_typ_wrt_typ_rec.
+  intros. apply trans_ftyp_open_typ_wrt_typ_rec.
 Qed.
 
-Theorem trans_typ_lc_ftyp : forall (A:typ),
-  lc_typ A -> lc_ftyp (trans_typ A).
+Theorem trans_ftyp_lc_ftyp : forall (A:typ),
+  lc_typ A -> lc_ftyp (trans_ftyp A).
 Proof.
   intros. induction H; simpl; eauto.
   - apply lc_ftyp_all. unfold open_ftyp_wrt_ftyp. simpl. eauto.
   - apply lc_ftyp_all. intros.
-    rewrite <- trans_typ_open_typ_wrt_typ with (A2 := (typ_var_f X)).
+    rewrite <- trans_ftyp_open_typ_wrt_typ with (A2 := (typ_var_f X)).
     auto.
 Qed.
 
-#[local] Hint Resolve trans_typ_lc_ftyp : core.
+#[local] Hint Resolve trans_ftyp_lc_ftyp : core.
 
 Theorem trans_env_notin_dom : forall Ψ X,
   X `notin` dom Ψ -> X `notin` dom ⟦ Ψ ⟧.
@@ -94,8 +94,8 @@ Proof.
   destruct a; destruct d; destruct_binds; auto.
 Qed.
 
-Theorem trans_typ_wf : forall Ψ A,
-  Ψ ᵗ⊢ᵈ A -> f_wf_typ (trans_env Ψ) (trans_typ A).
+Theorem trans_ftyp_wf : forall Ψ A,
+  Ψ ᵗ⊢ᵈ A -> f_wf_typ (trans_env Ψ) (trans_ftyp A).
 Proof.
   intros. induction H; simpl; eauto...
   - apply f_wf_typ__all with (L:=dom Ψ).
@@ -105,12 +105,12 @@ Proof.
   - apply f_wf_typ__tvar. apply trans_env_stvar_in. auto.
   - apply f_wf_typ__all with (L:= L `union` dom Ψ). 
     intros. inst_cofinites_with X.
-    rewrite trans_typ_open_typ_wrt_typ in H1. auto.
+    rewrite trans_ftyp_open_typ_wrt_typ in H1. auto.
 Qed.
 
 Theorem trans_env_wf_tenv_wf_fenv : forall Ψ,
   ⊢ᵈₜ Ψ -> f_wf_env ⟦ Ψ ⟧.
-Proof with eauto using trans_typ_wf.
+Proof with eauto using trans_ftyp_wf.
   intros. induction H; simpl; eauto...
   constructor...
   constructor... 
@@ -128,11 +128,11 @@ Inductive d_sub_elab : denv -> typ -> typ -> fexp -> Prop :=
   | d_sub_elab__top : forall (Ψ:denv) (A:typ),
       d_wf_env Ψ ->
       d_wf_typ Ψ A ->
-      d_sub_elab Ψ A typ_top (fexp_abs (trans_typ A) fexp_unit)
+      d_sub_elab Ψ A typ_top (fexp_abs (trans_ftyp A) fexp_unit)
   | d_sub_elab__bot : forall (Ψ:denv) (B:typ),
       d_wf_env Ψ ->
       d_wf_typ Ψ B ->
-      d_sub_elab Ψ typ_bot B (fexp_abs (ftyp_all (ftyp_var_b 0)) (fexp_tapp (fexp_var_b 0) (trans_typ B)))
+      d_sub_elab Ψ typ_bot B (fexp_abs (ftyp_all (ftyp_var_b 0)) (fexp_tapp (fexp_var_b 0) (trans_ftyp B)))
   | d_sub_elab__unit : forall (Ψ:denv),
       d_wf_env Ψ ->
       d_sub_elab Ψ typ_unit typ_unit (fexp_abs ftyp_unit (fexp_var_b 0))
@@ -144,8 +144,8 @@ Inductive d_sub_elab : denv -> typ -> typ -> fexp -> Prop :=
       d_sub_elab Ψ B1 A1 co1ᶠ ->
       d_sub_elab Ψ A2 B2 co2ᶠ ->
       d_sub_elab Ψ (typ_arrow A1 A2) (typ_arrow B1 B2)
-        (fexp_abs (ftyp_arrow (trans_typ A1) (trans_typ A2))
-                  (fexp_abs (trans_typ B1)
+        (fexp_abs (ftyp_arrow (trans_ftyp A1) (trans_ftyp A2))
+                  (fexp_abs (trans_ftyp B1)
                             (fexp_app co2ᶠ
                                       (fexp_app (fexp_var_b 1)
                                                 (fexp_app co1ᶠ (fexp_var_b 0))))))
@@ -154,46 +154,46 @@ Inductive d_sub_elab : denv -> typ -> typ -> fexp -> Prop :=
       ( forall X , X \notin L -> s_in X  (open_typ_wrt_typ  B   (typ_var_f X) ) ) ->
       ( forall X , X \notin L -> d_sub_elab  ( X ~ dbind_stvar_empty  ++  Ψ )   (open_typ_wrt_typ  A   (typ_var_f X) )   (open_typ_wrt_typ  B   (typ_var_f X) ) (open_fexp_wrt_ftyp coᶠ (ftyp_var_f X)) ) ->
       d_sub_elab Ψ (typ_all A) (typ_all B)
-        (fexp_abs (trans_typ (typ_all A)) (fexp_tabs (fexp_app coᶠ (fexp_tapp (fexp_var_b 0) (ftyp_var_b 0)))))
+        (fexp_abs (trans_ftyp (typ_all A)) (fexp_tabs (fexp_app coᶠ (fexp_tapp (fexp_var_b 0) (ftyp_var_b 0)))))
   | d_sub_elab__alll : forall (L:vars) (Ψ:denv) (A B T:typ) (coᶠ:fexp),
       d_wneq_all Ψ B ->
       ( forall X , X \notin L -> s_in X  (open_typ_wrt_typ  A   (typ_var_f X) ) ) ->
       d_mono_typ Ψ T ->
       d_sub_elab Ψ  (open_typ_wrt_typ  A   T )  B coᶠ ->
       d_sub_elab Ψ (typ_all A) B
-        (fexp_abs (trans_typ (typ_all A)) (fexp_app coᶠ (fexp_tapp (fexp_var_b 0) (trans_typ T))))
+        (fexp_abs (trans_ftyp (typ_all A)) (fexp_app coᶠ (fexp_tapp (fexp_var_b 0) (trans_ftyp T))))
   | d_sub_elab__intersection1 : forall (Ψ:denv) (A B1 B2:typ) (co1ᶠ co2ᶠ:fexp),
       d_sub_elab Ψ A B1 co1ᶠ ->
       d_sub_elab Ψ A B2 co2ᶠ ->
       d_sub_elab Ψ A (typ_intersection B1 B2)
-        (fexp_abs (trans_typ A)
+        (fexp_abs (trans_ftyp A)
                   (fexp_pair (fexp_app co1ᶠ (fexp_var_b 0))
                           (fexp_app co2ᶠ (fexp_var_b 0))))
   | d_sub_elab__intersection2 : forall (Ψ:denv) (A1 A2 B:typ) (coᶠ:fexp),
       d_sub_elab Ψ A1 B coᶠ ->
       d_wf_typ Ψ A2 ->
       d_sub_elab Ψ (typ_intersection A1 A2) B
-        (fexp_abs (trans_typ (typ_intersection A1 A2)) (fexp_app coᶠ (fexp_proj1 (fexp_var_b 0))))
+        (fexp_abs (trans_ftyp (typ_intersection A1 A2)) (fexp_app coᶠ (fexp_proj1 (fexp_var_b 0))))
   | d_sub_elab__intersection3 : forall (Ψ:denv) (A1 A2 B:typ) (coᶠ:fexp),
       d_sub_elab Ψ A2 B coᶠ ->
       d_wf_typ Ψ A1 ->
       d_sub_elab Ψ (typ_intersection A1 A2) B
-        (fexp_abs (trans_typ (typ_intersection A1 A2)) (fexp_app coᶠ (fexp_proj2 (fexp_var_b 0))))
+        (fexp_abs (trans_ftyp (typ_intersection A1 A2)) (fexp_app coᶠ (fexp_proj2 (fexp_var_b 0))))
   | d_sub_elab__union1 : forall (Ψ:denv) (A B1 B2:typ) (coᶠ:fexp),
       d_sub_elab Ψ A B1 coᶠ ->
       d_wf_typ Ψ B2 ->
       d_sub_elab Ψ A (typ_union B1 B2)
-        (fexp_abs (trans_typ A) (fexp_inl (fexp_app coᶠ (fexp_var_b 0))))
+        (fexp_abs (trans_ftyp A) (fexp_inl (fexp_app coᶠ (fexp_var_b 0))))
   | d_sub_elab__union2 : forall (Ψ:denv) (A B1 B2:typ) (coᶠ:fexp),
       d_sub_elab Ψ A B2 coᶠ ->
       d_wf_typ Ψ B1 ->
       d_sub_elab Ψ A (typ_union B1 B2)
-        (fexp_abs (trans_typ A) (fexp_inr (fexp_app coᶠ (fexp_var_b 0))))
+        (fexp_abs (trans_ftyp A) (fexp_inr (fexp_app coᶠ (fexp_var_b 0))))
   | d_sub_elab__union3 : forall (Ψ:denv) (A1 A2 B:typ) (co1ᶠ co2ᶠ:fexp),
       d_sub_elab Ψ A1 B co1ᶠ ->
       d_sub_elab Ψ A2 B co2ᶠ ->
       d_sub_elab Ψ (typ_union A1 A2) B
-        (fexp_abs (trans_typ (typ_union A1 A2)) (fexp_case (fexp_var_b 0) (fexp_app co1ᶠ (fexp_var_b 0)) (fexp_app co2ᶠ (fexp_var_b 0)))).
+        (fexp_abs (trans_ftyp (typ_union A1 A2)) (fexp_case (fexp_var_b 0) (fexp_app co1ᶠ (fexp_var_b 0)) (fexp_app co2ᶠ (fexp_var_b 0)))).
 
 Notation "Ψ ⊢ A <: B ↪ coᶠ" := (d_sub_elab Ψ A B coᶠ) (at level 65, A at next level, B at next level, no associativity) : type_scope.
 
@@ -208,32 +208,32 @@ Inductive d_infabs_elab : denv -> typ -> typ -> typ -> fexp -> Prop :=
       d_wf_typ Ψ A ->
       d_wf_typ Ψ B ->
       d_infabs_elab Ψ (typ_arrow A B) A B
-        (fexp_abs (trans_typ (typ_arrow A B)) (fexp_var_b 0))
+        (fexp_abs (trans_ftyp (typ_arrow A B)) (fexp_var_b 0))
   | d_infabs_elab__all : forall (Ψ:denv) (A B C T:typ) (coᶠ:fexp),
       d_mono_typ Ψ T -> 
       d_wf_typ Ψ (typ_all A) ->
       d_infabs_elab Ψ  (open_typ_wrt_typ  A   T ) B C coᶠ ->
       d_infabs_elab Ψ (typ_all A) B C
-        (fexp_abs (trans_typ (typ_all A))
-                  (fexp_app coᶠ (fexp_tapp (fexp_var_b 0) (trans_typ T))))
+        (fexp_abs (trans_ftyp (typ_all A))
+                  (fexp_app coᶠ (fexp_tapp (fexp_var_b 0) (trans_ftyp T))))
   | d_infabs_elab__intersection1 : forall (Ψ:denv) (A1 A2 B C:typ) (coᶠ:fexp),
       d_wf_typ Ψ A2 ->
       d_infabs_elab Ψ A1 B C coᶠ ->
       d_infabs_elab Ψ (typ_intersection A1 A2) B C
-        (fexp_abs (trans_typ (typ_intersection A1 A2))
+        (fexp_abs (trans_ftyp (typ_intersection A1 A2))
                   (fexp_app coᶠ (fexp_proj1 (fexp_var_b 0))))
   | d_infabs_elab__intersection2 : forall (Ψ:denv) (A1 A2 B C:typ) (coᶠ:fexp),
       d_wf_typ Ψ A1 ->
       d_infabs_elab Ψ A2 B C coᶠ ->
       d_infabs_elab Ψ (typ_intersection A1 A2) B C
-        (fexp_abs (trans_typ (typ_intersection A1 A2))
+        (fexp_abs (trans_ftyp (typ_intersection A1 A2))
                   (fexp_app coᶠ (fexp_proj2 (fexp_var_b 0))))
   | d_infabs_elab__union : forall (Ψ:denv) (A1 A2 B1 C1 B2 C2:typ) (co1ᶠ co2ᶠ:fexp),
       d_infabs_elab Ψ A1 B1 C1 co1ᶠ ->
       d_infabs_elab Ψ A2 B2 C2 co2ᶠ ->
       d_infabs_elab Ψ (typ_union A1 A2) (typ_intersection B1 B2) (typ_union C1 C2)
-        (fexp_abs (trans_typ (typ_union A1 A2))
-                  (fexp_abs (trans_typ (typ_intersection B1 B2))
+        (fexp_abs (trans_ftyp (typ_union A1 A2))
+                  (fexp_abs (trans_ftyp (typ_intersection B1 B2))
                             (fexp_case (fexp_var_b 1)
                                       (fexp_inl (fexp_app co1ᶠ (fexp_proj1 (fexp_var_b 1))))
                                       (fexp_inr (fexp_app co2ᶠ (fexp_proj2 (fexp_var_b 1))))))).
@@ -254,31 +254,31 @@ Inductive d_inftapp_elab : denv -> typ -> typ -> typ -> fexp -> fexp -> Prop :=
       d_wf_typ Ψ (typ_all A) ->
       d_wf_typ Ψ B ->
       d_inftapp_elab Ψ (typ_all A) B (open_typ_wrt_typ  A   B )  
-        (fexp_abs (trans_typ (typ_all A)) (fexp_var_b 0))
-        (fexp_abs (trans_typ (typ_all A)) (fexp_tapp (fexp_var_b 0) (trans_typ B)))
+        (fexp_abs (trans_ftyp (typ_all A)) (fexp_var_b 0))
+        (fexp_abs (trans_ftyp (typ_all A)) (fexp_tapp (fexp_var_b 0) (trans_ftyp B)))
   | d_inftapp_elab__intersection1 : forall (Ψ:denv) (A1 A2 B C1:typ) (co1ᶠ co2ᶠ:fexp),
       d_wf_typ Ψ A2 ->
       d_inftapp_elab Ψ A1 B C1 co1ᶠ co2ᶠ ->
       d_inftapp_elab Ψ (typ_intersection A1 A2) B C1
-        (fexp_abs (trans_typ (typ_intersection A1 A2))
+        (fexp_abs (trans_ftyp (typ_intersection A1 A2))
                   (fexp_app co1ᶠ (fexp_proj1 (fexp_var_b 0))))
         co2ᶠ
   | d_inftapp_elab__intersection2 : forall (Ψ:denv) (A1 A2 B C2:typ) (co1ᶠ co2ᶠ:fexp),
       d_wf_typ Ψ A1 ->
       d_inftapp_elab Ψ A2 B C2 co1ᶠ co2ᶠ ->
       d_inftapp_elab Ψ (typ_intersection A1 A2) B C2
-        (fexp_abs (trans_typ (typ_intersection A1 A2))
+        (fexp_abs (trans_ftyp (typ_intersection A1 A2))
                   (fexp_app co1ᶠ (fexp_proj2 (fexp_var_b 0))))
         co2ᶠ
   | d_inftapp_elab__union : forall (Ψ:denv) (A1 A2 B C1 C2:typ) (co1ᶠ co2ᶠ co3 co4:fexp),
       d_inftapp_elab Ψ A1 B C1 co1ᶠ co2ᶠ ->
       d_inftapp_elab Ψ A2 B C2 co3 co4 ->
       d_inftapp_elab Ψ (typ_union A1 A2) B (typ_union C1 C2)
-        (fexp_abs (trans_typ (typ_union A1 A2))
+        (fexp_abs (trans_ftyp (typ_union A1 A2))
                   (fexp_case (fexp_var_b 0)
                               (fexp_inl (fexp_app co2ᶠ (fexp_app co1ᶠ (fexp_var_b 0))))
                               (fexp_inr (fexp_app co4 (fexp_app co3 (fexp_var_b 0))))))
-        (fexp_abs (trans_typ (typ_union C1 C2)) (fexp_var_b 0)).
+        (fexp_abs (trans_ftyp (typ_union C1 C2)) (fexp_var_b 0)).
 
 Notation "Ψ ⊢ A ○ B ⇒⇒ C ↪ co1ᶠ | co2ᶠ" :=
     (d_inftapp_elab Ψ A B C co1ᶠ co2ᶠ) 
@@ -308,7 +308,7 @@ Inductive d_chk_inf_elab : denv -> exp -> typing_mode -> typ -> fexp -> Prop :=
       d_mono_typ Ψ (typ_arrow A B) ->
       ( forall x , x \notin  L  -> d_chk_inf_elab  ( x ~ (dbind_typ A)  ++  Ψ )  ( open_exp_wrt_exp e (exp_var_f x) ) typingmode__chk B (open_fexp_wrt_fexp eᶠ (fexp_var_f x)))  ->
       d_chk_inf_elab Ψ (exp_abs e) typingmode__inf (typ_arrow A B)
-        (fexp_abs (trans_typ A) eᶠ)
+        (fexp_abs (trans_ftyp A) eᶠ)
   | d_chk_inf_elab__inf_tabs : forall (L:vars) (Ψ:denv) (e:exp) (A:typ) (eᶠ:fexp),
       ( forall X , X \notin  L  -> s_in X (open_typ_wrt_typ A (typ_var_f X)))  ->
       ( forall X , X \notin  L  -> d_chk_inf_elab  ( X ~ dbind_tvar_empty  ++  Ψ ) ( open_exp_wrt_typ e (typ_var_f X) ) typingmode__chk ( open_typ_wrt_typ A (typ_var_f X) ) (open_fexp_wrt_ftyp eᶠ (ftyp_var_f X)))  ->
@@ -327,7 +327,7 @@ Inductive d_chk_inf_elab : denv -> exp -> typing_mode -> typ -> fexp -> Prop :=
       d_wf_typ Ψ A ->
       ( forall x , x \notin  L  -> d_chk_inf_elab  ( x ~ (dbind_typ A)  ++  Ψ )  ( open_exp_wrt_exp e (exp_var_f x) ) typingmode__chk B (open_fexp_wrt_fexp eᶠ (fexp_var_f x)))  ->
       d_chk_inf_elab Ψ (exp_abs e) typingmode__chk (typ_arrow A B)
-        (fexp_abs (trans_typ A) eᶠ)
+        (fexp_abs (trans_ftyp A) eᶠ)
   | d_chk_inf_elab__chk_sub : forall (Ψ:denv) (e:exp) ( A B:typ) (eᶠ coᶠ:fexp),
       d_chk_inf_elab Ψ e typingmode__inf A eᶠ ->
       d_sub_elab Ψ A B coᶠ ->
@@ -358,7 +358,7 @@ Proof.
   intros. induction H; eauto.
 Qed.
 
-Lemma trans_typ_rename_tvar : forall A X Y,
+Lemma trans_ftyp_rename_tvar : forall A X Y,
   subst_ftyp_in_ftyp (ftyp_var_f Y) X ᵗ⟦ A ⟧ = ᵗ⟦ {`Y ᵗ/ₜ X} A ⟧.
 Proof.
   intros. induction A; simpl; eauto.
@@ -375,14 +375,14 @@ Lemma d_sub_elab_rename_dtvar : forall Ψ1 Ψ2 A B b X Y coᶠ,
   Y ∉ (dom (Ψ2 ++ (X, b) :: Ψ1)) ->
   (map (subst_typ_in_dbind `Y X) Ψ2) ++ (Y , b) :: Ψ1  ⊢ {`Y ᵗ/ₜ X} A <: {`Y ᵗ/ₜ X} B ↪ subst_ftyp_in_fexp (ftyp_var_f Y) X coᶠ.
 Proof with eauto 6 using d_wf_typ_rename_dtvar, d_wf_env_rename_dtvar.
-  intros. dependent induction H0; eauto; try solve [simpl; repeat rewrite trans_typ_rename_tvar; eauto 6 using d_wf_typ_rename_dtvar, d_wf_env_rename_dtvar].
+  intros. dependent induction H0; eauto; try solve [simpl; repeat rewrite trans_ftyp_rename_tvar; eauto 6 using d_wf_typ_rename_dtvar, d_wf_env_rename_dtvar].
   - simpl. destruct_eq_atom; auto.
     + econstructor; eauto... destruct H; eauto.
     + econstructor; eauto...
       dependent destruction H0; apply binds_remove_mid in H; apply binds_app_iff in H; destruct H...
       * econstructor... apply binds_app_2. apply binds_map with (f:=(subst_typ_in_dbind ` Y X)) in H...
       * eapply d_wf_typ__stvar. apply binds_app_2. apply binds_map with (f:=(subst_typ_in_dbind ` Y X)) in H...
-  - simpl. repeat rewrite trans_typ_rename_tvar.
+  - simpl. repeat rewrite trans_ftyp_rename_tvar.
     replace (ftyp_all ᵗ⟦ {` Y ᵗ/ₜ X} A ⟧) with (ᵗ⟦ typ_all ( {` Y ᵗ/ₜ X} A ) ⟧) by auto.
     inst_cofinites_for d_sub_elab__all; intros; inst_cofinites_with X0; auto.
     + rewrite subst_typ_in_typ_open_typ_wrt_typ_fresh2...
@@ -395,7 +395,7 @@ Proof with eauto 6 using d_wf_typ_rename_dtvar, d_wf_env_rename_dtvar.
       * rewrite <- subst_ftyp_in_fexp_open_fexp_wrt_ftyp...
         rewrite_env (map (subst_typ_in_dbind ` Y X) (X0 ~ ■ ++ Ψ2) ++ (Y, b) :: Ψ1)...
       * simpl. destruct_eq_atom...
-  - simpl. repeat rewrite trans_typ_rename_tvar.
+  - simpl. repeat rewrite trans_ftyp_rename_tvar.
     inst_cofinites_for d_sub_elab__alll; intros; inst_cofinites_with X0; eauto...
     + eapply d_wneq_all_rename_dtvar; auto.
       eapply d_sub_elab_sound in H2.
@@ -405,9 +405,9 @@ Proof with eauto 6 using d_wf_typ_rename_dtvar, d_wf_env_rename_dtvar.
     + eapply d_mono_typ_rename_dtvar...
       apply d_sub_elab_sound in H2. apply d_sub_d_wf_env in H2...
     + rewrite <- subst_typ_in_typ_open_typ_wrt_typ...
-  - simpl; repeat rewrite trans_typ_rename_tvar... econstructor...
-  - simpl; repeat rewrite trans_typ_rename_tvar... econstructor...
-  - simpl; repeat rewrite trans_typ_rename_tvar... econstructor...
+  - simpl; repeat rewrite trans_ftyp_rename_tvar... econstructor...
+  - simpl; repeat rewrite trans_ftyp_rename_tvar... econstructor...
+  - simpl; repeat rewrite trans_ftyp_rename_tvar... econstructor...
 Qed.
 
 Lemma d_sub_elab_rename_tvar_cons : forall Ψ A B X Y coᶠ b,
@@ -441,7 +441,7 @@ Proof with auto.
   - pick fresh X. inst_cofinites_with_keep X.
     destruct H3 as [coᶠ ?].
     exists 
-      (fexp_abs (trans_typ (typ_all A)) (fexp_tabs (fexp_app (close_fexp_wrt_ftyp X coᶠ) (fexp_tapp (fexp_var_b 0) (ftyp_var_b 0))))).
+      (fexp_abs (trans_ftyp (typ_all A)) (fexp_tabs (fexp_app (close_fexp_wrt_ftyp X coᶠ) (fexp_tapp (fexp_var_b 0) (ftyp_var_b 0))))).
     inst_cofinites_for d_sub_elab__all; intros; inst_cofinites_with X0; auto.
     erewrite <- subst_typ_in_typ_open_typ_wrt_typ_tvar2 with (X:=X)...
     erewrite <- subst_typ_in_typ_open_typ_wrt_typ_tvar2 with (X:=X) (A:=B)...
@@ -486,10 +486,10 @@ Lemma d_infabs_elab_rename_tvar : forall Ψ1 Ψ2 X Y A B C coᶠ,
   (map (subst_typ_in_dbind (`Y) X) Ψ2) ++ (Y , □) :: Ψ1 ⊢ {`Y ᵗ/ₜ X} A ▹ {`Y ᵗ/ₜ X} B → {`Y ᵗ/ₜ X} C ↪ subst_ftyp_in_fexp (ftyp_var_f Y) X coᶠ.
 Proof with eauto.
   intros. dependent induction H; eauto; try solve [simpl; 
-    repeat rewrite trans_typ_rename_tvar; 
+    repeat rewrite trans_ftyp_rename_tvar; 
     try econstructor; 
     eauto 6 using d_wf_typ_rename_dtvar, d_mono_typ_rename_dtvar, d_wf_tenv_rename_tvar, d_wf_env_rename_dtvar].
-  - simpl. repeat rewrite trans_typ_rename_tvar.
+  - simpl. repeat rewrite trans_ftyp_rename_tvar.
     econstructor; eauto.
     + eapply d_mono_typ_rename_dtvar...
       eapply d_infabs_elab_sound in H1.
@@ -505,10 +505,10 @@ Lemma d_inftapp_elab_rename_tvar : forall Ψ1 Ψ2 X Y A B C co1ᶠ co2ᶠ,
   (map (subst_typ_in_dbind (`Y) X) Ψ2) ++ (Y , □) :: Ψ1 ⊢ {`Y ᵗ/ₜ X} A ○ {`Y ᵗ/ₜ X} B ⇒⇒ {`Y ᵗ/ₜ X} C ↪ subst_ftyp_in_fexp (ftyp_var_f Y) X co1ᶠ | subst_ftyp_in_fexp (ftyp_var_f Y) X co2ᶠ.
 Proof.
   intros. dependent induction H; eauto; try solve [simpl; 
-    repeat rewrite trans_typ_rename_tvar; 
+    repeat rewrite trans_ftyp_rename_tvar; 
     try econstructor; 
     eauto 6 using d_wf_typ_rename_dtvar, d_mono_typ_rename_dtvar, d_wf_tenv_rename_tvar, d_wf_env_rename_dtvar].
-  - simpl. repeat rewrite trans_typ_rename_tvar.
+  - simpl. repeat rewrite trans_ftyp_rename_tvar.
     rewrite subst_typ_in_typ_open_typ_wrt_typ; auto.
     econstructor; eauto using d_wf_typ_rename_dtvar, d_mono_typ_rename_dtvar, d_wf_tenv_rename_tvar, d_wf_env_rename_dtvar.
     replace (typ_all ({` Y ᵗ/ₜ X} A)) with ({` Y ᵗ/ₜ X} typ_all A) by auto.
@@ -521,11 +521,11 @@ Lemma d_chk_inf_elab_rename_tvar : forall Ψ1 Ψ2 X Y e A eᶠ mode,
   d_chk_inf_elab (map (subst_typ_in_dbind (`Y) X) Ψ2 ++ (Y, □) :: Ψ1) ({` Y ᵉ/ₜ X} e) mode ({` Y ᵗ/ₜ X} A) (subst_ftyp_in_fexp (ftyp_var_f Y) X eᶠ).
 Proof with eauto using d_wf_typ_rename_dtvar, d_mono_typ_rename_dtvar, d_wf_tenv_rename_tvar.
   intros. dependent induction H; 
-    try solve [simpl; repeat rewrite trans_typ_rename_tvar;
+    try solve [simpl; repeat rewrite trans_ftyp_rename_tvar;
                eauto using d_wf_typ_rename_dtvar, d_mono_typ_rename_dtvar, d_wf_tenv_rename_tvar, d_infabs_elab_rename_tvar].
   - simpl. econstructor; eauto...
     apply d_binds_var_typ_rename_tvar; eauto.
-  - simpl. repeat rewrite trans_typ_rename_tvar. 
+  - simpl. repeat rewrite trans_ftyp_rename_tvar. 
     inst_cofinites_for d_chk_inf_elab__inf_abs_mono; intros; inst_cofinites_with X0; eauto.
     + replace (typ_arrow ({` Y ᵗ/ₜ X} A) ({` Y ᵗ/ₜ X} B)) with ({` Y ᵗ/ₜ X} (typ_arrow A B)) by auto.
       eapply d_mono_typ_rename_dtvar; eauto.
@@ -537,7 +537,7 @@ Proof with eauto using d_wf_typ_rename_dtvar, d_mono_typ_rename_dtvar, d_wf_tenv
       replace (fexp_var_f x) with (subst_ftyp_in_fexp (ftyp_var_f Y) X (fexp_var_f x)) by auto.
       rewrite <- subst_ftyp_in_fexp_open_fexp_wrt_fexp.
       eapply H1; eauto.
-  - simpl. repeat rewrite trans_typ_rename_tvar. 
+  - simpl. repeat rewrite trans_ftyp_rename_tvar. 
     inst_cofinites_for d_chk_inf_elab__inf_tabs; intros; inst_cofinites_with X0; eauto. 
     + rewrite subst_typ_in_typ_open_typ_wrt_typ_fresh2...
       apply s_in_subst_inv...
@@ -546,11 +546,11 @@ Proof with eauto using d_wf_typ_rename_dtvar, d_mono_typ_rename_dtvar, d_wf_tenv
       replace (ftyp_var_f X0) with (subst_ftyp_in_ftyp (ftyp_var_f Y) X (ftyp_var_f X0)) by (simpl; destruct_eq_atom; auto).
       rewrite <- subst_ftyp_in_fexp_open_fexp_wrt_ftyp...
       rewrite_env (map (subst_typ_in_dbind (`Y) X) (X0 ~ □ ++ Ψ2) ++ (Y, □) :: Ψ1)...
-  - simpl. repeat rewrite trans_typ_rename_tvar.
+  - simpl. repeat rewrite trans_ftyp_rename_tvar.
     econstructor; eauto.
     + eapply d_wf_typ_rename_dtvar...
     + eapply d_inftapp_elab_rename_tvar; eauto.
-  - simpl. repeat rewrite trans_typ_rename_tvar. 
+  - simpl. repeat rewrite trans_ftyp_rename_tvar. 
     inst_cofinites_for d_chk_inf_elab__chk_abs_top eᶠ:=(subst_ftyp_in_fexp (ftyp_var_f Y) X eᶠ); intros; inst_cofinites_with x; eauto.
     replace (exp_var_f x) with ({` Y ᵉ/ₜ X} (exp_var_f x)) by auto.
     rewrite <- subst_typ_in_exp_open_exp_wrt_exp; eauto.
@@ -558,7 +558,7 @@ Proof with eauto using d_wf_typ_rename_dtvar, d_mono_typ_rename_dtvar, d_wf_tenv
     rewrite <- subst_ftyp_in_fexp_open_fexp_wrt_fexp; eauto.
     rewrite_env (map (subst_typ_in_dbind (`Y) X) (x ~ dbind_typ typ_bot ++ Ψ2) ++ (Y, □) :: Ψ1).
     eapply H0; eauto.
-  - simpl. repeat rewrite trans_typ_rename_tvar. 
+  - simpl. repeat rewrite trans_ftyp_rename_tvar. 
     inst_cofinites_for d_chk_inf_elab__chk_abs; eauto...
     + intros. inst_cofinites_with x.
       replace (exp_var_f x) with ({` Y ᵉ/ₜ X} (exp_var_f x)) by auto.
@@ -671,7 +671,7 @@ Proof.
   (* λx. e => τ1 -> τ2 *)
   - pick fresh x. inst_cofinites_with x.
     destruct H1 as [eᶠ].
-    exists (fexp_abs (trans_typ A) (close_fexp_wrt_fexp x eᶠ)).
+    exists (fexp_abs (trans_ftyp A) (close_fexp_wrt_fexp x eᶠ)).
     inst_cofinites_for d_chk_inf_elab__inf_abs_mono; eauto.
     intros. rewrite_close_open_subst.
     erewrite <- subst_exp_in_exp_open_exp_wrt_exp_var2; eauto.
@@ -698,13 +698,90 @@ Proof.
     eapply d_chk_inf_elab_rename_var_cons; eauto.
   - pick fresh x. inst_cofinites_with x.
     destruct H1 as [eᶠ].
-    exists (fexp_abs (trans_typ A1) (close_fexp_wrt_fexp x eᶠ)).
+    exists (fexp_abs (trans_ftyp A1) (close_fexp_wrt_fexp x eᶠ)).
     inst_cofinites_for d_chk_inf_elab__chk_abs; eauto.
     intros. rewrite_close_open_subst.
     erewrite <- subst_exp_in_exp_open_exp_wrt_exp_var2; eauto.
     eapply d_chk_inf_elab_rename_var_cons; eauto.
   - apply d_sub_elab_complete in H0.
     destruct_conj; eauto.
+Qed.
+
+
+
+Lemma d_sub_elab_lc_ftyp : forall Ψ A B coᶠ,
+  Ψ ⊢ A <: B ↪ coᶠ -> lc_ftyp (trans_ftyp A) /\ lc_ftyp (trans_ftyp B).
+Proof.
+  intros. apply d_sub_elab_sound in H.
+  apply d_sub_d_wf in H.
+  intuition; eauto using trans_ftyp_lc_ftyp.
+Qed.
+
+Lemma d_sub_elab_lc_ftyp1 : forall Ψ A B coᶠ,
+  Ψ ⊢ A <: B ↪ coᶠ -> lc_ftyp (trans_ftyp A).
+Proof.
+  intros. apply d_sub_elab_lc_ftyp in H. intuition.
+Qed.
+
+Lemma d_sub_elab_lc_ftyp2 : forall Ψ A B coᶠ,
+  Ψ ⊢ A <: B ↪ coᶠ -> lc_ftyp (trans_ftyp B).
+Proof.
+  intros. apply d_sub_elab_lc_ftyp in H. intuition.
+Qed.
+
+Ltac solve_lc_fexp :=
+  match goal with
+    | _ : _ |- forall x , _ => intros
+    | _ : _ |- context [open_fexp_wrt_fexp ?e1 ?e2] =>  unfold open_fexp_wrt_fexp; simpl; eauto
+    | _ : _ |- context [open_ftyp_wrt_ftyp ?A1 ?A2] =>  unfold open_ftyp_wrt_ftyp; simpl; eauto
+    | H : lc_fexp ?e |- context [open_fexp_wrt_fexp_rec ?n ?e1 ?e] => rewrite open_fexp_wrt_fexp_rec_lc_fexp; eauto
+  end.
+
+Ltac solve_lc_fexp_sub := 
+  repeat
+    try solve_lc_fexp;
+    try match goal with 
+      | H : ?Ψ ⊢ ?A <: ?B ↪ ?coᶠ |- lc_ftyp (trans_ftyp ?A) => eapply d_sub_elab_lc_ftyp1; eauto
+      | H : ?Ψ ⊢ ?A <: ?B ↪ ?coᶠ |- lc_ftyp (trans_ftyp ?B) => eapply d_sub_elab_lc_ftyp2; eauto
+    end;
+    econstructor;
+    eauto.
+
+Hint Extern 2 (lc_ftyp ?A) => solve_lc_fexp_sub : core.
+Hint Extern 1 (lc_fexp ?A) => solve_lc_fexp_sub : core.
+
+Theorem d_sub_elab_lc_fexp : forall Ψ A B coᶠ,
+  Ψ ⊢ A <: B ↪ coᶠ -> lc_fexp coᶠ.
+Proof with eauto.
+  intros. induction H...
+  - solve_lc_fexp_sub.
+    + simpl. pick fresh X. inst_cofinites_with X.
+      apply d_sub_elab_sound in H1.
+      apply d_sub_d_wf in H1. intuition.
+      apply d_wf_typ_lc_typ in H1.
+      eapply lc_ftyp_all_exists with (X1:=X)...
+      replace (ftyp_var_f X) with (trans_ftyp (typ_var_f X))...
+      rewrite <- trans_ftyp_open_typ_wrt_typ...
+    + intros. unfold open_fexp_wrt_fexp. simpl. 
+      pick fresh X. apply lc_fexp_tabs_exists with (X1:=X). 
+      unfold open_fexp_wrt_ftyp. simpl. constructor.
+      * inst_cofinites_with X.
+        apply degree_fexp_wrt_fexp_of_lc_fexp in H2 as Hdeg.
+        apply degree_fexp_wrt_fexp_open_fexp_wrt_ftyp_rec_inv_mutual in Hdeg.
+        rewrite open_fexp_wrt_fexp_rec_degree_fexp_wrt_fexp_mutual...
+      * solve_lc_fexp_sub.
+  - solve_lc_fexp_sub.
+    simpl. pick fresh X. inst_cofinites_with X. 
+    apply lc_ftyp_all_exists with (X1:=X)...
+    apply d_sub_elab_sound in H2.
+    apply d_sub_d_wf_typ1 in H2.
+    apply d_wf_typ_lc_typ in H2.
+    eapply lc_typ_open_stvar_subst_mono with (X:=X) in H2; eauto.
+    replace (ftyp_var_f X) with (trans_ftyp (typ_var_f X))...
+    rewrite <- trans_ftyp_open_typ_wrt_typ...
+  - simpl...
+  - simpl...
+  - simpl...
 Qed.
 
 Theorem d_sub_elab_sound_f : forall Ψ A B coᶠ,
@@ -755,7 +832,7 @@ Proof with eauto 6.
     eapply f_typing__app with (A1:=ᵗ⟦ A ᵗ^^ₜ T ⟧ ); eauto.
     + rewrite open_fexp_wrt_fexp_rec_lc_fexp; eauto.
       admit. admit.
-    + rewrite trans_typ_open_typ_wrt_typ. econstructor; eauto.
+    + rewrite trans_ftyp_open_typ_wrt_typ. econstructor; eauto.
       econstructor; eauto. admit.
   - inst_cofinites_for f_typing__abs; intros.
     simpl. unfold open_fexp_wrt_fexp. simpl...
@@ -838,7 +915,7 @@ Proof with eauto with safety.
     apply typing_tapp with (B1:=ftyp_var_b 0); eauto with safety.
     apply typing_var; eauto.
     apply wf_env_typ; eauto with safety.
-    apply trans_typ_wf with (Ψ:=Ψ) (T:=typ_all (typ_var_b 0)).
+    apply trans_ftyp_wf with (Ψ:=Ψ) (T:=typ_all (typ_var_b 0)).
     apply dwftyp_all with (L:=dom Ψ); unfold open_typ_wrt_typ; simpl; auto.
   - apply typing_abs with (L:=dom Ψ).
     unfold open_fexp_wrt_fexp. simpl. intros.
@@ -848,12 +925,12 @@ Proof with eauto with safety.
     unfold open_fexp_wrt_fexp. simpl. intros.
     apply typing_var; eauto.
     apply wf_env_typ; eauto with safety.
-    apply trans_typ_wf with (T:=typ_var_f X); auto.
+    apply trans_ftyp_wf with (T:=typ_var_f X); auto.
   - apply typing_abs with (L:=dom Ψ).
     unfold open_fexp_wrt_fexp. simpl. intros.
     apply typing_var; eauto.
     apply wf_env_typ; eauto with safety.
-    apply trans_typ_wf with (T:=typ_var_f SX); auto.
+    apply trans_ftyp_wf with (T:=typ_var_f SX); auto.
   - apply typing_abs with (L:=dom Ψ).
     unfold open_fexp_wrt_fexp. simpl. intros.
     apply typing_abs with (L:=dom Ψ `union` singleton x).
@@ -864,12 +941,12 @@ Proof with eauto with safety.
     { apply sub_elab_lc_fexp in H0. auto. }
     repeat rewrite open_fexp_wrt_fexp_rec_lc_fexp;
     try rewrite open_fexp_wrt_fexp_rec_lc_fexp; auto.
-    apply typing_app with (B1:=trans_typ A2).
+    apply typing_app with (B1:=trans_ftyp A2).
     + admit. (* weaken *)
-    + apply typing_app with (B1:=trans_typ A1).
+    + apply typing_app with (B1:=trans_ftyp A1).
     * apply typing_var; auto.
       admit. (* wf *)
-    * apply typing_app with (B1:=trans_typ B1).
+    * apply typing_app with (B1:=trans_ftyp B1).
       -- admit. (* weaken *)
       -- apply typing_var; auto.
        admit. (* wf *)
@@ -884,11 +961,11 @@ Proof with eauto with safety.
     try rewrite open_fexp_wrt_fexp_rec_lc_fexp; auto.
     repeat rewrite open_fexp_wrt_ftyp_rec_lc_fexp;
     try rewrite open_fexp_wrt_ftyp_rec_lc_fexp; auto.
-    replace (ftyp_var_f X) with (trans_typ (typ_var_f X)); auto.
-    apply typing_app with (B1:=trans_typ (A1 ᵗ^^ₜ typ_var_f X)).
-    + rewrite <- trans_typ_open_typ_wrt_typ with (B1:=B1) (B2:=typ_var_f X).
+    replace (ftyp_var_f X) with (trans_ftyp (typ_var_f X)); auto.
+    apply typing_app with (B1:=trans_ftyp (A1 ᵗ^^ₜ typ_var_f X)).
+    + rewrite <- trans_ftyp_open_typ_wrt_typ with (B1:=B1) (B2:=typ_var_f X).
     admit. (* weaken *)
-    + rewrite trans_typ_open_typ_wrt_typ.
+    + rewrite trans_ftyp_open_typ_wrt_typ.
     apply typing_tapp; eauto with safety.
     apply typing_var; auto.
     admit. (* wf *)
@@ -898,9 +975,9 @@ Proof with eauto with safety.
     { apply sub_elab_lc_fexp in H5. auto. }
     repeat rewrite open_fexp_wrt_fexp_rec_lc_fexp;
     try rewrite open_fexp_wrt_fexp_rec_lc_fexp; auto.
-    apply typing_app with (B1:=trans_typ (A1 ᵗ^^ₜ B2)).
+    apply typing_app with (B1:=trans_ftyp (A1 ᵗ^^ₜ B2)).
     + admit. (* weaken *)
-    + rewrite trans_typ_open_typ_wrt_typ.
+    + rewrite trans_ftyp_open_typ_wrt_typ.
     apply typing_tapp; eauto with safety.
     apply typing_var; auto.
     admit. (* wf *)
@@ -913,11 +990,11 @@ Proof with eauto with safety.
     repeat rewrite open_fexp_wrt_fexp_rec_lc_fexp;
     try rewrite open_fexp_wrt_fexp_rec_lc_fexp; auto.
     apply typing_pair.
-    + apply typing_app with (B1:=trans_typ A1).
+    + apply typing_app with (B1:=trans_ftyp A1).
       * admit. (* weaken *)
       * apply typing_var; auto.
         admit. (* wf *)
-    + apply typing_app with (B1:=trans_typ A1).
+    + apply typing_app with (B1:=trans_ftyp A1).
       * admit. (* weaken *)
       * apply typing_var; auto.
         admit. (* wf *)
@@ -927,9 +1004,9 @@ Proof with eauto with safety.
     { apply sub_elab_lc_fexp in H. auto. }
     repeat rewrite open_fexp_wrt_fexp_rec_lc_fexp;
     try rewrite open_fexp_wrt_fexp_rec_lc_fexp; auto.
-    apply typing_app with (B1:=trans_typ A1).
+    apply typing_app with (B1:=trans_ftyp A1).
     + admit. (* weaken *) 
-    + apply typing_proj1 with (B2:=trans_typ A2).
+    + apply typing_proj1 with (B2:=trans_ftyp A2).
     apply typing_var; auto.
     admit. (* wf *)
   - apply typing_abs with (L:=dom Ψ).
@@ -938,9 +1015,9 @@ Proof with eauto with safety.
     { apply sub_elab_lc_fexp in H. auto. }
     repeat rewrite open_fexp_wrt_fexp_rec_lc_fexp;
     try rewrite open_fexp_wrt_fexp_rec_lc_fexp; auto.
-    apply typing_app with (B1:=trans_typ A2).
+    apply typing_app with (B1:=trans_ftyp A2).
     + admit. (* weaken *) 
-    + apply typing_proj2 with (B1:=trans_typ A1).
+    + apply typing_proj2 with (B1:=trans_ftyp A1).
     apply typing_var; auto.
     admit. (* wf *)
   - apply typing_abs with (L:=dom Ψ).
@@ -950,7 +1027,7 @@ Proof with eauto with safety.
     repeat rewrite open_fexp_wrt_fexp_rec_lc_fexp;
     try rewrite open_fexp_wrt_fexp_rec_lc_fexp; auto.
     apply typing_inl.
-    + eapply typing_app with (B1:=trans_typ A1).
+    + eapply typing_app with (B1:=trans_ftyp A1).
       * admit. (* weaken *)
       * apply typing_var; auto.
         admit. (* wf *)
@@ -962,7 +1039,7 @@ Proof with eauto with safety.
     repeat rewrite open_fexp_wrt_fexp_rec_lc_fexp;
     try rewrite open_fexp_wrt_fexp_rec_lc_fexp; auto.
     apply typing_inr.
-    + eapply typing_app with (B1:=trans_typ A1).
+    + eapply typing_app with (B1:=trans_ftyp A1).
       * admit. (* weaken *)
       * apply typing_var; auto.
         admit. (* wf *)
@@ -975,18 +1052,18 @@ Proof with eauto with safety.
     { apply sub_elab_lc_fexp in H0. auto. }
     repeat rewrite open_fexp_wrt_fexp_rec_lc_fexp;
     try rewrite open_fexp_wrt_fexp_rec_lc_fexp; auto.
-    apply typing_case with (B1:=trans_typ A1) (B2:=trans_typ A2)
+    apply typing_case with (B1:=trans_ftyp A1) (B2:=trans_ftyp A2)
                (L:=dom Ψ `union` singleton x).
     + apply typing_var; auto. admit. (* wf *) 
     + intros. unfold open_fexp_wrt_fexp. simpl.
     rewrite open_fexp_wrt_fexp_rec_lc_fexp; auto.
-    apply typing_app with (B1:=trans_typ A1).
+    apply typing_app with (B1:=trans_ftyp A1).
       * admit. (* weaken *) 
       * apply typing_var; auto.
         admit. (* wf *) 
     + intros. unfold open_fexp_wrt_fexp. simpl.
     rewrite open_fexp_wrt_fexp_rec_lc_fexp; auto.
-    apply typing_app with (B1:=trans_typ A2).
+    apply typing_app with (B1:=trans_ftyp A2).
       * admit. (* weaken *) 
       * apply typing_var; auto.
         admit. (* wf *) 
@@ -1012,12 +1089,12 @@ Proof.
     rewrite open_fexp_wrt_fexp_rec_lc_fexp; auto.
   - apply lc_ftyp_prod.
     + admit.
-    + apply trans_typ_lc_ftyp. apply d_wf_typ_lc_typ with (Ψ:=Ψ); auto.
+    + apply trans_ftyp_lc_ftyp. apply d_wf_typ_lc_typ with (Ψ:=Ψ); auto.
   - unfold open_fexp_wrt_fexp. simpl. intros.
     apply lc_fexp_app; eauto with safety.
     rewrite open_fexp_wrt_fexp_rec_lc_fexp; auto.
   - apply lc_ftyp_prod.
-    + apply trans_typ_lc_ftyp. apply d_wf_typ_lc_typ with (Ψ:=Ψ); auto.
+    + apply trans_ftyp_lc_ftyp. apply d_wf_typ_lc_typ with (Ψ:=Ψ); auto.
     + admit.
   - unfold open_fexp_wrt_fexp. simpl. intros.
     apply lc_fexp_app; eauto with safety.
@@ -1026,7 +1103,7 @@ Admitted.
 
 Theorem infabs_sound_f : forall Ψ A B C Co,
   d_infabs_elab Ψ A B C Co ->
-  typing (trans_env Ψ) Co (ftyp_arrow (trans_typ A) (ftyp_arrow (trans_typ B) (trans_typ C))).
+  typing (trans_env Ψ) Co (ftyp_arrow (trans_ftyp A) (ftyp_arrow (trans_ftyp B) (trans_ftyp C))).
 Proof with eauto with safety.
   intros. induction H; simpl; eauto.
   - apply typing_abs with (L:=dom Ψ).
@@ -1046,28 +1123,28 @@ Proof with eauto with safety.
     assert (Hlc: lc_fexp Co).
     { apply d_infabs_elab__lc_fexp in H2. auto. }
     rewrite open_fexp_wrt_fexp_rec_lc_fexp; auto.
-    apply typing_app with (B1:=trans_typ (open_typ_wrt_typ B1 B2)).
+    apply typing_app with (B1:=trans_ftyp (open_typ_wrt_typ B1 B2)).
     + admit. (* weaken *)
-    + rewrite trans_typ_open_typ_wrt_typ. apply typing_tapp.
-      * apply trans_typ_lc_ftyp; auto.
+    + rewrite trans_ftyp_open_typ_wrt_typ. apply typing_tapp.
+      * apply trans_ftyp_lc_ftyp; auto.
       * apply typing_var; auto. admit. (* wf *)
   - apply typing_abs with (L:=dom Ψ).
     unfold open_fexp_wrt_fexp. simpl. intros.
     assert (Hlc: lc_fexp Co).
     { apply d_infabs_elab__lc_fexp in H0. auto. }
     rewrite open_fexp_wrt_fexp_rec_lc_fexp; auto.
-    apply typing_app with (B1:=trans_typ B1); auto.
+    apply typing_app with (B1:=trans_ftyp B1); auto.
     + admit. (* weaken *)
-    + apply typing_proj1 with (B2:=trans_typ B2).
+    + apply typing_proj1 with (B2:=trans_ftyp B2).
       apply typing_var; auto. admit. (* wf *)
   - apply typing_abs with (L:=dom Ψ).
     unfold open_fexp_wrt_fexp. simpl. intros.
     assert (Hlc: lc_fexp Co).
     { apply d_infabs_elab__lc_fexp in H0. auto. }
     rewrite open_fexp_wrt_fexp_rec_lc_fexp; auto.
-    apply typing_app with (B1:=trans_typ B2); auto.
+    apply typing_app with (B1:=trans_ftyp B2); auto.
     + admit. (* weaken *)
-    + apply typing_proj2 with (B1:=trans_typ B1).
+    + apply typing_proj2 with (B1:=trans_ftyp B1).
       apply typing_var; auto. admit. (* wf *)
   - apply typing_abs with (L:=dom Ψ).
     unfold open_fexp_wrt_fexp. simpl. intros.
@@ -1081,22 +1158,22 @@ Proof with eauto with safety.
     repeat rewrite open_fexp_wrt_fexp_rec_lc_fexp; auto.
     apply typing_case with
       (L:=dom Ψ `union` singleton x `union` singleton x0)
-      (B1:=trans_typ B1) (B2:=trans_typ B2).
+      (B1:=trans_ftyp B1) (B2:=trans_ftyp B2).
     + apply typing_var; auto. admit. (* wf *)
     + unfold open_fexp_wrt_fexp. simpl. intros.
       rewrite open_fexp_wrt_fexp_rec_lc_fexp; auto.
       apply typing_inl.
-      * apply typing_app with (B1:=trans_typ T3).
+      * apply typing_app with (B1:=trans_ftyp T3).
         -- admit. (* weaken *)
-        -- apply typing_proj1 with (B2:=trans_typ T5).
+        -- apply typing_proj1 with (B2:=trans_ftyp T5).
            apply typing_var; auto. admit. (* wf *)
       * admit. (* wf *)
     + unfold open_fexp_wrt_fexp. simpl. intros.
       rewrite open_fexp_wrt_fexp_rec_lc_fexp; auto.
       apply typing_inr.
-      * apply typing_app with (B1:=trans_typ T5).
+      * apply typing_app with (B1:=trans_ftyp T5).
         -- admit. (* weaken *)
-        -- apply typing_proj2 with (B1:=trans_typ T3).
+        -- apply typing_proj2 with (B1:=trans_ftyp T3).
            apply typing_var; auto. admit. (* wf *)
       * admit. (* wf *)
 Admitted.
@@ -1108,19 +1185,19 @@ Proof.
   - split; apply lc_fexp_abs; eauto with safety;
     unfold open_fexp_wrt_fexp; simpl; auto.
   - split; apply lc_fexp_abs; eauto with safety.
-    + replace (ftyp_all (trans_typ B1)) with (trans_typ (typ_all B1)); eauto.
-      apply trans_typ_lc_ftyp. eauto.
+    + replace (ftyp_all (trans_ftyp B1)) with (trans_ftyp (typ_all B1)); eauto.
+      apply trans_ftyp_lc_ftyp. eauto.
     + unfold open_fexp_wrt_fexp. simpl. auto.
-    + replace (ftyp_all (trans_typ B1)) with (trans_typ (typ_all B1)); eauto.
-      apply trans_typ_lc_ftyp. eauto.
+    + replace (ftyp_all (trans_ftyp B1)) with (trans_ftyp (typ_all B1)); eauto.
+      apply trans_ftyp_lc_ftyp. eauto.
     + unfold open_fexp_wrt_fexp. simpl. intros.
-      apply lc_fexp_tapp; eauto. apply trans_typ_lc_ftyp. eauto. 
+      apply lc_fexp_tapp; eauto. apply trans_ftyp_lc_ftyp. eauto. 
 Admitted.
 
 Theorem inftapp_sound_f : forall Ψ A B C co1ᶠ co2ᶠ,
   d_inftapp_elab Ψ A B C co1ᶠ co2ᶠ -> exists D,
-  typing (trans_env Ψ) co1ᶠ (ftyp_arrow (trans_typ A) D) /\
-    typing (trans_env Ψ) co2ᶠ (ftyp_arrow D (trans_typ C)).
+  typing (trans_env Ψ) co1ᶠ (ftyp_arrow (trans_ftyp A) D) /\
+    typing (trans_env Ψ) co2ᶠ (ftyp_arrow D (trans_ftyp C)).
 Proof with eauto with safety.
   intros. induction H; simpl; eauto.
   - exists (ftyp_all (ftyp_var_b 0)). split.
@@ -1130,15 +1207,15 @@ Proof with eauto with safety.
     + apply typing_abs with (L:=dom Ψ).
       unfold open_fexp_wrt_fexp. simpl. intros.
       apply typing_var; auto. admit. (* wf *)
-  - exists (ftyp_all (trans_typ B1)). split.
+  - exists (ftyp_all (trans_ftyp B1)). split.
     + apply typing_abs with (L:=dom Ψ).  
       unfold open_fexp_wrt_fexp. simpl. intros.
       apply typing_var; auto. admit. (* wf *)
     + apply typing_abs with (L:=dom Ψ).  
       unfold open_fexp_wrt_fexp. simpl. intros.
-      rewrite trans_typ_open_typ_wrt_typ.
+      rewrite trans_ftyp_open_typ_wrt_typ.
       apply typing_tapp.
-      * apply trans_typ_lc_ftyp. eauto.
+      * apply trans_ftyp_lc_ftyp. eauto.
       * apply typing_var; auto. admit. (* wf *)
   - inversion IHinftapp_elab. destruct H2.
     exists x. split.
@@ -1148,9 +1225,9 @@ Proof with eauto with safety.
       { apply d_inftapp_elab__lc_fexp in H1. auto. }
       destruct Hlc as [Hlc1 Hlc2].
       rewrite open_fexp_wrt_fexp_rec_lc_fexp; auto.
-      apply typing_app with (B1:=trans_typ A1).
+      apply typing_app with (B1:=trans_ftyp A1).
       * admit. (* weaken *)
-      * apply typing_proj1 with (B2:=trans_typ A2).
+      * apply typing_proj1 with (B2:=trans_ftyp A2).
         apply typing_var; auto. admit. (* wf *)
     + auto.
   - inversion IHinftapp_elab. destruct H2.
@@ -1161,14 +1238,14 @@ Proof with eauto with safety.
       { apply d_inftapp_elab__lc_fexp in H1. auto. }
       destruct Hlc as [Hlc1 Hlc2].
       rewrite open_fexp_wrt_fexp_rec_lc_fexp; auto.
-      apply typing_app with (B1:=trans_typ A2).
+      apply typing_app with (B1:=trans_ftyp A2).
       * admit. (* weaken *)
-      * apply typing_proj2 with (B1:=trans_typ A1).
+      * apply typing_proj2 with (B1:=trans_ftyp A1).
         apply typing_var; auto.  admit. (* wf *)
     + auto.
   - inversion IHinftapp_elab1. inversion IHinftapp_elab2.
     destruct H1. destruct H2.
-    exists (trans_typ (typ_intersection C1 C2)). split.
+    exists (trans_ftyp (typ_intersection C1 C2)). split.
     + apply typing_abs with (L:=dom Ψ).
       unfold open_fexp_wrt_fexp. simpl. intros.
       assert (Hlc12: lc_fexp co1ᶠ /\ lc_fexp co2ᶠ).
@@ -1181,22 +1258,22 @@ Proof with eauto with safety.
       apply typing_pair.
       * apply typing_app with (B1:=x).
         -- admit. (* weaken *) 
-        -- apply typing_app with (B1:=trans_typ A1).
+        -- apply typing_app with (B1:=trans_ftyp A1).
            ++ admit. (* weaken *)
-           ++ apply typing_proj1 with (B2:=trans_typ A2).
+           ++ apply typing_proj1 with (B2:=trans_ftyp A2).
               apply typing_var; auto. admit. (* wf *)
       * apply typing_app with (B1:=x0).
         -- admit. (* weaken *) 
-        -- apply typing_app with (B1:=trans_typ A2).
+        -- apply typing_app with (B1:=trans_ftyp A2).
            ++ admit. (* weaken *)
-           ++ apply typing_proj2 with (B1:=trans_typ A1).
+           ++ apply typing_proj2 with (B1:=trans_ftyp A1).
               apply typing_var; auto. admit. (* wf *)
     + apply typing_abs with (L:=dom Ψ).
       unfold open_fexp_wrt_fexp. simpl. intros.
       apply typing_var; auto. admit. (* wf *)
   - inversion IHinftapp_elab1. inversion IHinftapp_elab2.
     destruct H1. destruct H2.
-    exists (trans_typ (typ_union C1 C2)). split.
+    exists (trans_ftyp (typ_union C1 C2)). split.
     + apply typing_abs with (L:=dom Ψ).
       unfold open_fexp_wrt_fexp. simpl. intros.
       assert (Hlc12: lc_fexp co1ᶠ /\ lc_fexp co2ᶠ).
@@ -1207,14 +1284,14 @@ Proof with eauto with safety.
       destruct Hlc34 as [Hlc3 Hlc4].
       repeat rewrite open_fexp_wrt_fexp_rec_lc_fexp; auto.
       apply typing_case with (L:=dom Ψ `union` singleton x1)
-        (B1:=trans_typ A1) (B2:=trans_typ A2).
+        (B1:=trans_ftyp A1) (B2:=trans_ftyp A2).
       * apply typing_var; auto. admit. (* wf *)
       * unfold open_fexp_wrt_fexp. simpl. intros.
         repeat rewrite open_fexp_wrt_fexp_rec_lc_fexp; auto.
         apply typing_inl.
         -- apply typing_app with (B1:=x).
            ++ admit. (* weaken *) 
-           ++ apply typing_app with (B1:=trans_typ A1).
+           ++ apply typing_app with (B1:=trans_ftyp A1).
               ** admit. (* weaken *)
               ** apply typing_var; auto. admit. (* wf *)
         -- admit. (* wf *)
@@ -1223,7 +1300,7 @@ Proof with eauto with safety.
         apply typing_inr.
         -- apply typing_app with (B1:=x0).
            ++ admit. (* weaken *) 
-           ++ apply typing_app with (B1:=trans_typ A2).
+           ++ apply typing_app with (B1:=trans_ftyp A2).
               ** admit. (* weaken *)
               ** apply typing_var; auto. admit. (* wf *)
         -- admit. (* wf *)
@@ -1233,7 +1310,7 @@ Proof with eauto with safety.
 Admitted.
 
 Theorem trans_binds : forall Ψ x T,
-  binds x (dbind_typ T) Ψ -> binds x (bind_typ (trans_typ T)) (trans_env Ψ).
+  binds x (dbind_typ T) Ψ -> binds x (bind_typ (trans_ftyp T)) (trans_env Ψ).
 Proof.
   intros. induction Ψ; auto.
   inversion H.
@@ -1249,23 +1326,23 @@ Proof.
 Admitted.
 
 Theorem typing_sound_f : forall Ψ e T C mode,
-  d_chk_inf_elab Ψ e mode T C -> typing (trans_env Ψ) C (trans_typ T).
+  d_chk_inf_elab Ψ e mode T C -> typing (trans_env Ψ) C (trans_ftyp T).
 Proof.
   intros. induction H; simpl; eauto.
   - apply typing_var; auto. admit. (* wf *)
     apply trans_binds. auto.
-  - apply typing_app with (B1:=trans_typ B2); auto.
-    apply typing_app with (B1:=trans_typ B1); auto.
+  - apply typing_app with (B1:=trans_ftyp B2); auto.
+    apply typing_app with (B1:=trans_ftyp B1); auto.
     apply infabs_sound_f; auto.
   - apply typing_tabs with (L:=L `union` dom Ψ).
     unfold open_fexp_wrt_ftyp. simpl. intros.
     inst_cofinites_with X. assert (Hlc: lc_fexp C).
     { apply d_chk_inf_elab__lc_fexp in H0. auto. }
     rewrite open_fexp_wrt_ftyp_rec_lc_fexp; auto.
-    rewrite <- trans_typ_open_typ_wrt_typ with (B2:=typ_var_f X). auto.
+    rewrite <- trans_ftyp_open_typ_wrt_typ with (B2:=typ_var_f X). auto.
   - apply inftapp_sound_f in H1. destruct H1. destruct H1.
     apply typing_app with (B1:=x); auto.
-    apply typing_app with (B1:=trans_typ B1); auto.
+    apply typing_app with (B1:=trans_ftyp B1); auto.
   - apply typing_abs with (L:=L `union` dom Ψ).
     unfold open_fexp_wrt_ftyp. simpl. intros.
     inst_cofinites_with x. assert (Hlc: lc_fexp C).
@@ -1276,7 +1353,7 @@ Proof.
     inst_cofinites_with X. assert (Hlc: lc_fexp C).
     { apply d_chk_inf_elab__lc_fexp in H0. auto. }
     rewrite open_fexp_wrt_ftyp_rec_lc_fexp; auto.
-    rewrite <- trans_typ_open_typ_wrt_typ with (B2:=typ_var_f X). auto.
-  - eapply typing_app with (B1:=trans_typ A1); auto.
+    rewrite <- trans_ftyp_open_typ_wrt_typ with (B2:=typ_var_f X). auto.
+  - eapply typing_app with (B1:=trans_ftyp A1); auto.
     apply sub_sound_f. auto.
 Admitted. *)
